encode.v
@@ -3,93 +3,6 @@ Require Import ast_instructions.
 Require Import binary.
 Import ListNotations.
 
-Check (1,2).
-Check pair nat nat.
-Definition tag_opcode_assoc :=
-  list (tag * nat).
-
-Scheme Equality for list.
-Check list_beq.
-
-
-
-
-
-
-(* actually this is a good name for this function :p *)
-Fixpoint lookup (t : tag) (l : tag_opcode_assoc) : option nat :=
-  match l with
-    | [] => None
-    | (t',n) :: tl => if tag_beq t t'
-                      then Some n
-                      else lookup t tl
-  end.
-(* actually this is a good name for this function :p *)
-Fixpoint lookdown (n : nat) (l : tag_opcode_assoc) : option tag :=
-  match l with
-    | [] => None
-    | (t,n') :: tl => if  eqb n n'
-                      then Some t
-                      else lookdown n tl
-  end.
-
-(* this table is an association list of type tag_opcode_assoc with every associations that can be made in our langage *)
-Definition encdec : tag_opcode_assoc := [(tag_n(ADD),1);(tag_n(AND),2);(tag_i(ADD_I),3);(tag_i(AND_I),4)].
-
-Theorem lookup_encdec : forall (t : tag), exists n,
-                          lookup t encdec = Some n.
-Proof.
-  destruct t.
-  -destruct t.
-   +simpl. exists 1. reflexivity.
-   +simpl. exists 2. reflexivity.
-  -destruct t.
-   +simpl. exists 3. reflexivity.
-   +simpl. exists 4. reflexivity.
-Qed.
-
-
-(* TODO : i know that i can refoctor this proof but at the first try i didn't succeed so will try later *)
-Theorem look_up_down_encdec : forall (n : nat) (t : tag),
-                                lookup t encdec = Some n -> lookdown n encdec = Some t.
-Proof.
-  assert (I : forall (n : nat) (t : tag), lookup t encdec = Some n -> lookdown n encdec = Some t).
-  {
-    destruct t.
-    -destruct t.
-     +intros H.
-      simpl in H.
-      inversion H.
-      reflexivity.
-     +intros H.
-      simpl in H.
-      inversion H.
-      reflexivity.
-    -destruct t.
-     +intros H.
-      simpl in H.
-      inversion H.
-      reflexivity.
-     +intros H.
-      simpl in H.
-      inversion H.
-      reflexivity.
-  }
-  exact I.
-Qed.
-
-(* if i wan't it's very easy to proof with forall t exists n but this theorem is better and actually it's true *)
-Theorem look_down_up_encdec : forall (n : nat) (t : tag),
-                                lookdown n encdec = Some t -> lookup t encdec = Some n.
-Proof.
- (*  assert (I : forall (t : tag) (n : nat), lookdown n encdec = Some t -> lookup t encdec = Some n).
-  {
-
-       
-     
-  }*)
-  
-Admitted.
 
 
 
@@ -101,23 +14,31 @@ Definition operand_to_bin (o : operand) : option (list bool) :=
     | reg k => n_bit 8 k
     | empty => n_bit 8 0
   end.
-
-Definition encode (i : instruction) : binary_instruction :=
-  match lookup i.instr_opcode with
-    | some k => match n_bit 8 k with
-                  | some code => match operand_to_bin i.instr_operande1 with
-                                   | some o1 => match operand_to_bin i.instr_operande2 with
-                                                  | some o2 => match operand_to_bin i.instr_operande3 with
-                                                                 | some o3 => concat code (concat o1 (concat o2 o3)) 
-                                                                 | none => none
-                                                               end
-                                                  | none => none
-                                                end
-                                   | none => none
-                                 end
-                  | none => none
-                end
-    | none => None
+                
+(* TODO :: here i know that i can always get a binary_instruction but some function don't allow me to 
+return a binary_instruction without encapsulate it into an option type *)
+Definition encode_bis (i : instruction) : option binary_instruction :=
+  match i with
+    | mk_instr t op1 op2 op3 =>
+      match lookup t encdec with
+        | Some k => match n_bit 8 k with
+                      | Some code => match operand_to_bin op1 with
+                                       | Some o1 => match operand_to_bin op2 with
+                                                      | Some o2 => match operand_to_bin op3 with
+                                                                     | Some o3 => Some (code ++ o1 ++ o2 ++ o3)
+                                                                     | None => None
+                                                                   end
+                                                      | None => None
+                                                    end
+                                       | None => None
+                                     end
+                      | None => None
+                    end
+        | None => None
+      end
   end.
+
+
+
 
                 
